<section xml:id="section-week10-activity">
  <title>Week 10 Activity</title>
  <subsection xml:id="subsection-activity-eigenvalues">
    <title>Eigenvalues and Eigenvectors</title>
    <activity>
      <statement>
        <p>
          Calculate the eigenvalue and eigenvectors of this matrix.
          (Give the solutions in exact value). 
          <me>
            \left( \begin{matrix}
              -2 \amp 0 \amp 1 \\
              0 \amp -2 \amp 1 \\
              1 \amp 1 \amp 0 
            \end{matrix} \right) 
          </me>
        </p>
      </statement>
      <solution>
        <p>
          We follow the algorithm for eigenvalue and eigenvectors. The
          first step is writing the matrix <m>M - \lambda \Id</m>. 
          <me>
            \left( \begin{matrix}
              -2 - \lambda \amp 0 \amp 1 \\
              0 \amp -2 - \lambda \amp 1 \\
              1 \amp 1 \amp - \lambda 
            \end{matrix} \right) 
          </me>
          Then we calculate the determinant of this matrix. We use
          cofactor expansion on the first row.
          <md>
            <mrow>
              \amp \left| \begin{matrix}
                -2 - \lambda \amp 0 \amp 1 \\
                0 \amp -2 - \lambda \amp 1 \\
                1 \amp 1 \amp - \lambda 
              \end{matrix} \right| 
            </mrow>
            <mrow>
              \amp = 
              (1)(-2 - \lambda) \left| \begin{matrix}
                -2 - \lambda \amp 1 \\
                1 \amp -\lambda
              \end{matrix} \right| + 
              (-1)(0) \left| \begin{matrix}
                0 \amp 1 \\
                1 \amp -\lambda
              \end{matrix} \right| + 
              (1)(1) \left| \begin{matrix}
                0 \amp -2 - \lambda \\
                1 \amp 1 
              \end{matrix} \right| 
            </mrow>
            <mrow>
              \amp = (-2 - \lambda) \left[ (-2 - \lambda)(-\lambda) -
              1 \right] + 0 + \left[ (0)(1) - (-2 - \lambda)(1)
              \right] 
            </mrow>
            <mrow>
              \amp = (-2 - \lambda)(\lambda^2 + 2 \lambda - 1) + 2 +
              \lambda 
            </mrow>
            <mrow>
              \amp = -\lambda^3 - 2\lambda^2 - 2\lambda^2 - 4\lambda +
              \lambda + 2 + 2 + \lambda 
            </mrow>
            <mrow>
              \amp = -\lambda^3 - 4\lambda^2 - 2\lambda + 4
            </mrow>
          </md>
          By inspection or by computer, we can see that <m>\lambda =
          -2</m> is a root, so this polynomial factors as 
          <me>
            -\lambda^3 - 4\lambda^2 - 2\lambda + 4 = -(\lambda +
            2)(\lambda^2 + 2 \lambda - 2) 
          </me>.
          The quadratic piece does not factor into integer roots. The
          quadratic formula gives the other roots as <m>\lambda = -1
          \pm \sqrt{3}</m>. Now we find the kernel of each <m>M -
          \lambda Id</m> to calculate the matching eigenvectors. Let's
          start with <m>\lambda = -2</m>.
          <md>
            <mrow>
              \amp \left( \begin{array}{ccc|c}
                0 \amp 0 \amp 1 \amp 0 \\
                0 \amp 0 \amp 1 \amp 0 \\
                1 \amp 1 \amp 2 \amp 0 
              \end{array} \right)   
            </mrow>
            <mrow>
              \amp \text{We row reduce to find the kernel.}
            </mrow>
            <mrow>
              \amp \left( \begin{array}{ccc|c}
                1 \amp 1 \amp 0 \amp 0 \\
                0 \amp 0 \amp 1 \amp 0 \\
                0 \amp 0 \amp 0 \amp 0
              \end{array} \right)   
            </mrow>
            <mrow>
              \amp \Ker \left( \begin{matrix}
                0 \amp 0 \amp 1 \\
                0 \amp 0 \amp 1 \\
                1 \amp 1 \amp 2
              \end{matrix} \right) = \Span \left\{ \left( \begin{matrix}
                1 \\ -1 \\ 0 
              \end{matrix} \right) \right\}
            </mrow>
          </md>
          That gives us an eigenvector for <m>\lambda = -2</m>. 
          Next, let's look at <m>\lambda = -1 + \sqrt{3}</m>.
          <md>
            <mrow>
              \amp \left( \begin{array}{ccc|c}
                -1 - \sqrt{3} \amp 0 \amp 1 \amp 0 \\
                0 \amp -1 - \sqrt{3} \amp 1 \amp 0 \\
                1 \amp 1 \amp 1 - \sqrt{3} \amp 0  
              \end{array} \right)   
            </mrow>
            <mrow>
              \amp \text{We row reduce to find the kernel.}
            </mrow>
            <mrow>
              \amp \left( \begin{array}{ccc|c}
                1 \amp 0 \amp \frac{-1}{1 + \sqrt{3}} \amp 0 \\
                0 \amp 1 \amp \frac{-1}{1 + \sqrt{3}} \amp 0 \\
                0 \amp 0 \amp 0 \amp 0  
              \end{array} \right)   
            </mrow>
            <mrow>
              \amp \Ker \left( \begin{matrix}
                -1 - \sqrt{3} \amp 0 \amp 1 \\
                0 \amp -1 - \sqrt{3} \amp 1 \\
                1 \amp 1 \amp 1 - \sqrt{3} 
              \end{matrix} \right) = \Span \left\{ \left( \begin{matrix}
                1 \\ 1 \\ 1 + \sqrt{3} 
              \end{matrix} \right) \right\}
            </mrow>
          </md>
          That gives us an eigenvector for <m>\lambda = -1 + \sqrt{3}</m>. 
          Next, let's look at <m>\lambda = -1 - \sqrt{3}</m>.
          <md>
            <mrow>
              \amp \left( \begin{array}{ccc|c}
                -1 + \sqrt{3} \amp 0 \amp 1 \\
                0 \amp -1 + \sqrt{3} \amp 1 \\
                1 \amp 1 \amp 1 + \sqrt{3} 
              \end{array} \right)   
            </mrow>
            <mrow>
              \amp \text{We row reduce to find the kernel.}
            </mrow>
            <mrow>
              \amp \left( \begin{array}{ccc|c}
                1 \amp 0 \amp \frac{-1}{1 - \sqrt{3}} \\
                0 \amp 1 \amp \frac{-1}{1 - \sqrt{3}} \\
                1 \amp 1 \amp 1 + \sqrt{3} 
              \end{array} \right)   
            </mrow>
            <mrow>
              \amp \Ker \left( \begin{matrix}
                -1 + \sqrt{3} \amp 0 \amp 1 \\
                0 \amp -1 + \sqrt{3} \amp 1 \\
                1 \amp 1 \amp 1 + \sqrt{3} 
              \end{matrix} \right) = \Span \left\{ \left( \begin{matrix}
                1 \amp 1 \amp 1 - \sqrt{3} 
              \end{matrix} \right) \right\}
            </mrow>
          </md>
          This gives us an eigenvector for <m>\lambda = -1 - \sqrt{3}</m>. 
        </p>
      </solution>
    </activity>
    <activity>
      <statement>
        <p>
          Calculate the eigenvalue and eigenvectors of this matrix.
          (Give the solutions in exact value). 
          <me>
            \left( \begin{matrix}
              0 \amp -6 \amp 0 \amp 6 \\
              0 \amp -2 \amp 0 \amp 2 \\
              0 \amp 0 \amp 2 \amp 2 \\
              0 \amp 0 \amp 0 \amp 2 
            \end{matrix} \right) 
          </me>
        </p>
      </statement>
      <solution>
        <p>
          We follow the algorithm for eigenvalue and eigenvectors. The
          first step is writing the matrix <m>M - \lambda \Id</m>. 
          <me>
            \left( \begin{matrix}
              -\lambda \amp -6 \amp 0 \amp 6 \\
              0 \amp -2 - \lambda \amp 0 \amp 2 \\
              0 \amp 0 \amp 2 - \lambda \amp 2 \\
              0 \amp 0 \amp 0 \amp 2 - \lambda 
            \end{matrix} \right) 
          </me>
          Then we calculate the determinant of this matrix. This is an
          upper triangular matrix, so the determinant is the product
          of the diagonal entries.
          <me>
            \left| \begin{matrix}
              -\lambda \amp -6 \amp 0 \amp 6 \\
              0 \amp -2 - \lambda \amp 0 \amp 2 \\
              0 \amp 0 \amp 2 - \lambda \amp 2 \\
              0 \amp 0 \amp 0 \amp 2 - \lambda 
              \end{matrix} \right| = -\lambda(-2 - \lambda)(2 -
              \lambda)^2 
          </me>
          This already in factor form, so we see that the eigenvalue
          are <m>\lambda = 0</m>, <m>\lambda = 2</m> and <m>\lambda =
          -2</m>. For each eigenvalue, we find the kernel of <m>M -
          \lambda \Id</m> to calculate the eigenvalues. Let's start
          with <m>\lambda = 0</m>
          <md>
            <mrow>
              \amp \left( \begin{array}{cccc|c}
                0 \amp -6 \amp 0 \amp 6 \amp 0 \\
                0 \amp -2 \amp 0 \amp 2 \amp 0 \\
                0 \amp 0 \amp 2 \amp 2 \amp 0 \\
                0 \amp 0 \amp 0 \amp 2 \amp 0 
              \end{array} \right)   
            </mrow>
            <mrow>
              \amp \text{We row reduce to find the kernel.}
            </mrow>
            <mrow>
              \amp \left( \begin{array}{cccc|c}
                0 \amp 1 \amp 0 \amp 0 \amp 0 \\
                0 \amp 0 \amp 1 \amp 0 \amp 0 \\
                0 \amp 0 \amp 0 \amp 1 \amp 0 \\
                0 \amp 0 \amp 0 \amp 0 \amp 0 
              \end{array} \right)   
            </mrow>
            <mrow>
              \amp \Ker \left( \begin{matrix}
                0 \amp -6 \amp 0 \amp 6 \\
                0 \amp -2 \amp 0 \amp 2 \\
                0 \amp 0 \amp 2 \amp 2 \\
                0 \amp 0 \amp 0 \amp 2 
              \end{matrix} \right) = \Span \left\{ \left( \begin{matrix}
                1 \\ 0 \\ 0 \\ 0 
              \end{matrix} \right) \right\}
            </mrow>
          </md>
          That gives us an eigenvector for <m>\lambda = 0</m>. 
          Next, let's look at <m>\lambda = 2</m>.
          <md>
            <mrow>
              \amp \left( \begin{array}{cccc|c}
                -2 \amp -6 \amp 0 \amp 6 \amp 0 \\
                0 \amp -4 \amp 0 \amp 2 \amp 0 \\
                0 \amp 0 \amp 0 \amp 2 \amp 0 \\
                0 \amp 0 \amp 0 \amp 0 \amp 0 
              \end{array} \right)   
            </mrow>
            <mrow>
              \amp \text{We row reduce to find the kernel.}
            </mrow>
            <mrow>
              \amp \left| \begin{array}{cccc|c}
                1 \amp 0 \amp 0 \amp 0 \amp 0 \\
                0 \amp 1 \amp 0 \amp 0 \amp 0 \\
                0 \amp 0 \amp 0 \amp 1 \amp 0 \\
                0 \amp 0 \amp 0 \amp 0 \amp 0 
              \end{array} \right)   
            </mrow>
            <mrow>
              \amp \Ker \left( \begin{matrix}
                -2 \amp -6 \amp 0 \amp 6 \\
                0 \amp -4 \amp 0 \amp 2 \\
                0 \amp 0 \amp 0 \amp 2 \\
                0 \amp 0 \amp 0 \amp 0 
              \end{matrix} \right) = \Span \left\{ \left( \begin{matrix}
                0 \\ 0 \\ 1 \\ 0 
              \end{matrix} \right) \right\}
            </mrow>
          </md>
          That gives us an eigenvector for <m>\lambda = 2</m>. 
          Next, let's look at <m>\lambda = -2</m>.
          <md>
            <mrow>
              \amp \left( \begin{array}{cccc|c}
                2 \amp -6 \amp 0 \amp 6 \amp 0 \\
                0 \amp 0 \amp 0 \amp 2 \amp 0 \\
                0 \amp 0 \amp 4 \amp 2 \amp 0 \\
                0 \amp 0 \amp 0 \amp 4 \amp 0 
              \end{array} \right)   
            </mrow>
            <mrow>
              \amp \text{We row reduce to find the kernel.}
            </mrow>
            <mrow>
              \amp \left| \begin{array}{cccc|c}
                1 \amp -3 \amp 0 \amp 0 \amp 0 \\
                0 \amp 0 \amp 1 \amp 0 \amp 0 \\
                0 \amp 0 \amp 0 \amp 1 \amp 0 \\
                0 \amp 0 \amp 0 \amp 0 \amp 0 
              \end{array} \right)   
            </mrow>
            <mrow>
              \amp \Ker \left( \begin{matrix}
                2 \amp -6 \amp 0 \amp 6 \\
                0 \amp 0 \amp 0 \amp 2 \\
                0 \amp 0 \amp 4 \amp 2 \\
                0 \amp 0 \amp 0 \amp 4 
              \end{matrix} \right) = \Span \left\{ \left( \begin{matrix}
                -3 \\ 1 \\ 0 \\ 0 
              \end{matrix} \right) \right\}
            </mrow>
          </md>
          This gives us an eigenvector for <m>\lambda = -2</m>. 
        </p>
      </solution>
    </activity>
    <activity>
      <statement>
        <p>
          Calculate the eigenvalues and eigenvectors of this matrix.
          Use approximate values (to three significant figures), but
          show all the steps in the algorithm.
          <me>
            \left( \begin{matrix} 
              0.294 \amp 0.343 \amp 0.945 \amp 0 \\
              0.812 \amp 0 \amp 0.310 \amp 0.050 \\
              0.110 \amp 0.745 \amp 0.901 \amp 0.874 \\
              0.314 \amp 0 \amp 0 \amp 0.041 
            \end{matrix} \right)
          </me>
        </p>
      </statement>
      <solution>
        <p>
          We ask a computer for the determinant of <m>M - \lambda
          Id</m>.
          <md>
            <mrow>
              \amp \left| \begin{matrix} 
                0.294 - \lambda \amp 0.343 \amp 0.945 \amp 0 \\
                0.812 \amp - \lambda \amp 0.310 \amp 0.050 \\
                0.110 \amp 0.745 \amp 0.901 - \lambda \amp 0.874 \\
                0.314 \amp 0 \amp 0 \amp 0.041 - \lambda  
              \end{matrix} \right| 
            </mrow>
            <mrow>
              \amp = x^4 - 1.235 x^3 - 0.300x^2 -
              0.515x - 0.025
            </mrow>
          </md>
          We ask a computer for the roots of this polynomial. There
          are two real roots: <m>\lambda = 1.622</m> and <m>\lambda =
          -0.049</m>. We calculate the kernel of <m>M - \lambda
          \Id</m> for both eigenvalues. We start with <m>\lambda =
          1.622</m>
          <md>  
            <mrow>
              \amp \Ker \left( \begin{matrix}
                -1.328 \amp 0.343 \amp 0.945 \amp 0 \\
                0.812 \amp -1.622 \amp 0.310 \amp 0.050 \\
                0.110 \amp 0.745 \amp -0.721 \amp 0.874 \\
                0.314 \amp 0 \amp 0 \amp -1.581 
              \end{matrix} \right) 
            </mrow>
            <mrow>
              \amp = \Span \left\{ \left( \begin{matrix}
                5.035 \\ 3.651 \\ 5.752 \\ 1
              \end{matrix} \right) \right\} 
            </mrow>
          </md>
          This gives us an eigevalue for <m>\lambda = 1.622</m>. Then
          we do the same for <m>\lambda = -0.049</m>. 
          <md>  
            <mrow>
              \amp \Ker \left( \begin{matrix}
                0.343 \amp 0.343 \amp 0.945 \amp 0 \\
                0.812 \amp 0.049\amp 0.310 \amp 0.050 \\
                0.110 \amp 0.745 \amp 0.950 \amp 0.874 \\
                0.314 \amp 0 \amp 0 \amp 0.090
              \end{matrix} \right) 
            </mrow>
            <mrow>
              \amp = \Span \left\{ \left( \begin{matrix}
               -0.286 \\ -2.351 \\ 0.957 \\ 1
              \end{matrix} \right) \right\} 
            </mrow>
          </md>
          This is an eigenvalue for <m>\lambda = -0.049</m>.
        </p>
      </solution>
    </activity>
    <activity>
      <statement>
        <p>
          Calculate the eigenvalues and eigenvectors of this matrix.
          Use approximate values (to three significant figures), but
          show all the steps in the algorithm.
          <me>
            \left( \begin{matrix} 
              2.30 \amp -0.29 \amp -0.92 \amp -3.17 \\
              -1.01 \amp 1.31 \amp 3.51 \amp 4.52 \\
              -3.68 \amp -5.42 \amp 8.54 \amp -4.62 \\
              -9.54 \amp -3.33 \amp -7.54 \amp 2.50 
            \end{matrix} \right)
          </me>
        </p>
      </statement>
      <solution>
        <p>
          We ask a computer for the determinant of <m>M - \lambda
          Id</m>.
          <md>
            <mrow>
              \amp \left| \begin{matrix} 
                2.30 - \lambda \amp -0.29 \amp -0.92 \amp -3.17 \\
                -1.01 \amp 1.31  - \lambda\amp 3.51 \amp 4.52 \\
                -3.68 \amp -5.42 \amp 8.54  - \lambda\amp -4.62 \\
                -9.54 \amp -3.33 \amp -7.54 \amp 2.50 - \lambda 
              \end{matrix} \right| 
            </mrow>
            <mrow>
              \amp = x^4 - 14.65 x^3 - 29.54 x^2 -
              35.81 x + 73.34
            </mrow>
          </md>
          We ask a computer for the roots of this polynomial. There
          are two real roots: <m>\lambda = 12.47</m> and <m>\lambda =
          2.26</m>. We calculate the kernel of <m>M - \lambda
          \Id</m> for both eigenvalues. We start with <m>\lambda =
          12.47</m>
          <md>  
            <mrow>
              \amp \Ker \left( \begin{matrix}
                -10.17\amp -0.29 \amp -0.92 \amp -3.17 \\
                -1.01 \amp -11.16 \amp 3.51 \amp 4.52 \\
                -3.68 \amp -5.42 \amp -4.02 \amp -4.62 \\
                -9.54 \amp -3.33 \amp -7.54 \amp -9.97
              \end{matrix} \right) 
            </mrow>
            <mrow>
              \amp = \Span \left\{ \left( \begin{matrix}
                -0.22 \\ 0.08 \\ -1.09 \\ 1 
              \end{matrix} \right) \right\} 
            </mrow>
          </md>
          This gives us an eigevalue for <m>\lambda = 12.47</m>. Then
          we do the same for <m>\lambda = 2.26</m>. 
          <md>  
            <mrow>
              \amp \Ker \left( \begin{matrix}
                0.04 \amp -0.29 \amp -0.92 \amp -3.17 \\
                -1.01 \amp -0.95 \amp 3.51 \amp 4.52 \\
                -3.68 \amp -5.42 \amp 6.28 \amp -4.62
                -9.54 \amp -3.33 \amp -7.54 \amp 0.24
              \end{matrix} \right) 
            </mrow>
            <mrow>
              \amp = \Span \left\{ \left( \begin{matrix}
                3.15 \\ -5.01 \\ 01.74 \\ 1 
              \end{matrix} \right) \right\} 
            </mrow>
          </md>
          This is an eigenvalue for <m>\lambda = 2.26</m>.
        </p>
      </solution>
    </activity>
  </subsection>
  <subsection xml:id="subsection-week10-proofs">
    <title>Proof Questions</title>
    <activity>
      <statement>
        <p>
          Prove that a square matrix <m>M</m> is invertible if and
          only if <m>\lambda = 0</m> is <emph>not</emph> an eigenvalue
          of <m>M</m>.
        </p>
      </statement>
      <solution>
        <p>
        </p>
      </solution>
    </activity>
    <activity>
      <statement>
        <p>
          Let <m>M</m> be an invertible matrix. Prove that
          <m>\lambda</m> is an eigenvalue of <m>M</m> if and only
          <m>\frac{1}{\lambda</m> is an eigenvalue of <m>M^{-1}</m>.
        </p>
      </statement>
      <solution>
        <p>
        </p>
      </solution>
    </activity>
    <activity>
      <statement>
        <p>
          Let <m>M</m> be a <m>3 \times 3</m> matrix. Prove that
          <m>M</m> has at least one real eigenvalue. 
        </p>
      </statement>
      <solution>
        <p>
        </p>
      </solution>
    </activity>
    <activity>
      <statement>
        <p>
          Prove that rotations in <m>\RR^2</m> has no real
          eigenvalues. 
        </p>
      </statement>
      <solution>
        <p>
        </p>
      </solution>
    </activity>
    <activity>
      <statement>
        <p>
          Prove that reflections in <m>\RR^2</m> have 1 and
          <m>(-1)</m> as their two eigenvalue and that their
          eigenvectors are perpendicular. Also argue that these two
          condition completely describe reflections (i.e., any matrix
          with these two properties must be a reflection). 
        </p>
      </statement>
      <solution>
        <p>
        </p>
      </solution>
    </activity>
  </subsection>
  <subsection xml:id="subsection-week1-concepts">
    <title>Conceptual Review Questions</title>
    <p>
      <ul>
        <li>
          What are eigenvalues and eigenvectors?
        </li>
        <li>
          How to determinants help to calculate eigenvalues?
        </li>
        <li>
          What is an eigenspace? What is a spectrum?
        </li>
      </ul>
    </p>
  </subsection>
</section>
