<section xml:id="week1-activity">
  <title>Week 1 Activity</title>
  <subsection xml:id="equations-of-lines">
    <title>Equations of Lines</title>
    <activity>
      <statement>
        <p>
          Find the equation of the line through the point
          <m>(3,2)</m> with slope 5.  
        </p>
      </statement>
      <solution>
        <p>
          Since the slope of the line is 5, using the slope intercept
          form, the equation of the line must be <m>y = 5x + b</m>.
          The only remaining unknown in this expression is the
          intercept <m>b</m>. We can solve for this <m>b</m> by
          inserting the point into the equation.
          <me>
            y = 5x + b \implies 2 = 5(3) + b \implies b = 2 - 15 = -13
          </me>
          Therefore, the equation of the line is <m>y = 5x-13</m>.
        </p>
      </solution>
    </activity>
    <activity>
      <statement>
        <p>
          Find the equation of the line through the point
          <m>(-2,-5)</m> with slope <m>\frac{1}{3}</m>.  
        </p>
      </statement>
      <solution>
        <p>
          Since the slope of the line is <m>/frac{1}{3}</m>,  using
          the slope intercept form, the equation of the line must be
          <m>y = \frac{1}{3}x + b</m>.  The only remaining unknown in
          this expression is the intercept <m>b</m>. We can solve for
          this <m>b</m> by inserting the point into the equation.
          <me>
            -5 = \frac{1}{3}(-2) + b \implies -5 = \frac{-2}{3} + b
            \implies b = -5 + \frac{2}{3} = \frac{-13}{3} 
          </me>
          Therefore, the equation of the line is <m>y =
          \frac{1}{3}x-\frac{13}{3}</m>.
        </p>
      </solution>
    </activity>
    <activity>
      <statement>
        <p>
          Find the equation of the line through the point
          <m>(\pi,1)</m> with slope <m>\frac{-1}{2}</m>.  
        </p>
      </statement>
      <solution>
        <p>
          Since the slope of the line is <m>\frac{-1}{2}</m>, using
          the slope intercept form, the equation of the line must be
          <m>y = \frac{-1}{2}x + b</m>.  The only remaining unknown in
          this expression is the intercept <m>b</m>. We can solve for
          this <m>b</m> by inserting the point into the equation.
          <me>
            y = \frac{-1}{2} x + b \implies 1 = \frac{-1}{2} \pi + b
            \implies b = 1 + \frac{\pi}{2} 
          </me>
          Therefore, the equation of the line is <m>y = \frac{-1}{2}x
          + 1 + \frac{\pi}{2}</m>. You might ask if there is an easier
          way to write this <m>b</m> value. We could express it as a
          decimal: it is approximately 2.57. However, that's less
          precise than simply writing <m>1 + \frac{\pi}{2}</m>, so I
          prefer to write it this way. 
        </p>
      </solution>
    </activity>
    <activity>
      <statement>
        <p>
          Find the equation of the line through the points
          <m>(0,4))</m> and <m>(2,2)</m>. 
        </p>
      </statement>
      <solution>
        <p>
          We need to calculate the slope first: this is calculate as
          the difference in the <m>y</m> coordinates divided by the
          difference in the <m>x</m> coordinates, often referred to as
          rise over run. 
          <me>
            m = \frac{4-2}{0-2} = \frac{2}{-2} = -1 
          </me>
          When we have the slope, we can use the slope intercept form,
          so the equation of the line will be <m>y = (-1)x + b</m>.
          Then we can use either of the points in this equation to
          solve for <m>b</m>. (Either point should give the same
          intercept; if they don't, we've made an error somewhere). 
          <me>
            y = -x + b \implies 4 = -0 + b \implies b = 4 
          </me>
          The equation of the line is <m>y = -x + 4</m>. 
        </p>
      </solution>
    </activity>
    <activity>
      <statement>
        <p>
          Find the equation of the line through the points
          <m>(-2,6))</m> and <m>(3,2)</m>. 
        </p>
      </statement>
      <solution>
        <p>
          We need to calculate the slope first: this is calculate as
          the difference in the <m>y</m> coordinates divided by the
          difference in the <m>x</m> coordinates, often referred to as
          rise over run. 
          <me>
            m = \frac{6-2}{(-2)-3} = \frac{4}{-5} = \frac{-4}{5} 
          </me>
          When we have the slope, we can use the slope intercept form,
          so the equation of the line will be <m>y = \frac{-4}{5}x +
          b</m>.  Then we can use either of the points in this
          equation to solve for <m>b</m>. (Either point should give
          the same intercept; if they don't, we've made an error
          somewhere).
          <me>
            y = \frac{-4}{5}x + b \implies 2 = \frac{-4}{5} (3) + b
            \implies 2 = \frac{-12}{5} + b \implies b = 2 +
            \frac{12}{5} = \frac{22}{5}
          </me>
          The equation of the line is <m>y = \frac{-4}{5}x +
          \frac{22}{5}</m>. 
        </p>
      </solution>
    </activity>
    <activity>
      <statement>
        <p>
          Find the equation of the line through the points
          <m>(\sqrt{2},3))</m> and <m>(2\sqrt{2},4)</m>. 
        </p>
      </statement>
      <solution>
        <p>
          We need to calculate the slope first: this is calculate as
          the difference in the <m>y</m> coordinates divided by the
          difference in the <m>x</m> coordinates, often referred to as
          rise over run. 
          <me>
            m = \frac{4-3}{2\sqrt{2} - \sqrt{2}} = \frac{1}{\sqrt{2}}
          </me>
          When we have the slope, we can use the slope intercept form,
          so the equation of the line will be <m>y =
          \frac{1}{\sqrt{2}} x + b</m>.
          Then we can use either of the points in this equation to
          solve for <m>b</m>. (Either point should give the same
          intercept; if they don't, we've made an error somewhere). 
          <me>
            y = \frac{1}{\sqrt{2}} x + b \implies 3 =
            \frac{1}{\sqrt{2}} (\sqrt{2}) + b \implies 3 = 1 + b
            \implies b = 3 - 1 = 2
          </me>
          The equation of the line is <m>y = \frac{1}{\sqrt{2}}x +
          2</m>.
        </p>
      </solution>
    </activity>
  </subsection>
  <subsection xml:id="equations-of-conics">
    <title>Equations of Conics</title>
    <activity>
      <statement>
        <p>
          Write the equation of an ellipse centred at the origin with
          semi-major axis 4 and semi-minor axis 2. 
        </p>
      </statement>
      <solution>
        <p>
          The standard form of the equation of an ellipse centred at
          the origin is <m> \frac{x^2}{a^2} + \frac{y^2}{b^2} = 1</m>
          where <m>a</m> and <m>b</m> are the semi-axes in the
          <m>x</m> and <m>y</m> directions, respectively. We've been
          told in the equation that the semi-major axis is 4 and the
          semi-minor axis is 2; but the question didn't specify which
          was the horizontal and which was the vertical directly.
          Therefore, we can just choose: setting <m>a=2</m> and
          <m>b=4</m> or vice-versa. 
          <me>
            \frac{x^2}{4} + \frac{y^2}{16} = 1 \text{ or }
            \frac{x^2}{16} + \frac{y^2}{4} = 1 \text{ or }
          </me>
        </p>
      </solution>
    </activity>
    <activity>
      <statement>
        <p>
          Write the equation of the circle centred at the origin with
          radius <m>\sqrt{15}</m>.
        </p>
      </statement>
      <solution>
        <p>
          The standard form of the equation of an ellipse centred at
          the origin is <m>x^2 + y^2 = r^2</m>. We are given the
          radius of <m>\sqrt{15}</m>, so we just square that value in
          insert it in the equation.
          <me>
            x^2 + y^2 = 15
          </me>
        </p>
      </solution>
    </activity>
    <activity>
      <statement>
        <p>
          Write the equation of the parabola with vertex <m>(3,-2)</m>
          and leading coefficient <m>\frac{1}{4}</m>.
        </p>
      </statement>
      <solution>
        <p>
          The standard form of the equation of an parabola with vertex
          <m>(c,d)</m> and leading coefficient <m>a</m> is <m>y = a (x
          - c)^2 + d </m>. We can just replace the three unknown with
          what we are given in the problem.
          <me>
            y = \frac{1}{4} (x-3)^2 - 2 
          </me>
          If we want a more conventional equation for this parabola,
          we can expand.
          <me>
            y = \frac{1}{4} (x^2 - 6x + 9) - 2 = \frac{1}{4} x^2 -
            \frac{3}{2} x + \frac{9}{4} 
          </me>
        </p>
      </solution>
    </activity>
  </subsection>
  <subsection xml:id="intersections">
    <title>Intersection of Lines and Conics</title>
    <activity>
      <statement>
        <p>
          Find the intersection of the line <m>y = -2x -5</m> and the
          line <m>y = 9x+1</m>. 
        </p>
      </statement>
      <solution>
        <p>
          Solving for intesection is algebraically the same as solving
          the system of two equations. In these two equations, the
          <m>y</m> terms are already isolated, so we can simply equate
          these two terms and solve for <m>x</m>. 
          <md>
            <mrow>
            -2x - 5 \amp = 9x + 1
            </mrow>
            <mrow>
            -2x - 9x \amp = 5 + 1
            </mrow>
            <mrow>
            -11x \amp = 6 \implies x = \frac{-6}{11}
            </mrow>
          </md>
          Then we can insert this <m>x</m> value into either equation
          to get the <m>y</m> value of the intersection point. (Either
          equation will give the same <m>y</m> value; if they don't,
          we've made an error somewhere). 
          <me>
            y = 9x + 1 = 9 \frac{-6}{11} + 1 = \frac{-54}{11} +
            \frac{11}{11} = \frac{-43}{11}
          </me>
          We conclude that the intersection point is <m> \left(
          \frac{-6}{11}, \frac{-43}{11} \right)</m>
        </p>
      </solution>
    </activity>
    <activity>
      <statement>
        <p>
          Find the intersection of the line <m>3x-2y+4=0</m> and the
          line <m>y = 4</m>. 
        </p>
      </statement>
      <solution>
        <p>
          Solving for intesection is algebraically the same as solving
          the system of two equations. In the second equation,
          <m>y</m> is already isolated, so we can replace <m>y</m> in
          the first equation. 
          <md>
            <mrow>
            3x - 2y + 4 \amp = 0 
            </mrow>
            <mrow>
            3x - 2(4) + 4 \amp = 0
            </mrow>
            <mrow>
            3x - 4 \amp = 0 \implies x = \frac{4}{3}
            </mrow>
          </md>
          We already know that <m>y</m> value must be 4, so this gives
          us the intersection point: <m>\left( \frac{4}{3}, 4
          \right)</m>.
        </p>
      </solution>
    </activity>
    <activity>
      <statement>
        <p>
          Find the intersection of the line <m>3y - x - 5 = 0</m> and
          the circle <m>x^2 + y^2 = 25</m>.
        </p>
      </statement>
      <solution>
        <p>
          Solving for intesection is algebraically the same as solving
          the system of two equations. If we isolate <m>x</m> in the
          first equation, we get <m>x = 3y - 5</m>. We can use this to
          replace <m>x</m> in the second equation and expand to get a
          quadratic equation.
          <md>
            <mrow>
            \left( 3y - 5 \right)^2 + y^2 \amp = 25
            </mrow>
            <mrow>
            9y^2 - 30y + 25 + y^2 \amp = 25
            </mrow>
            <mrow>
            10y^2 - 30 y \amp = 0 
            </mrow>
            <mrow>
            10y(y - 3) \amp = 0 
            </mrow>
          </md>
          The roots of the quadratic are 0 and 3, so those are the
          <m>y</m> values of the intersection points. We can use
          either equation to calculate the matching <m>x</m> values,
          but if we use the islated version of the first equation,
          that is most efficient.
          <md>
            <mrow>
            y \amp = 0 \implies x = 3y - 5 = 3(0) - 5 = -5 
            </mrow>
            <mrow>
            y \amp = 3 \implies x = 3y - 5 = 3(3) - 5 = 4
            </mrow>
          </md>
          Therefore, the two intersection point are <m>(-5, 0)</m> and
          <m>(4,3)</m>. 
        </p>
      </solution>
    </activity>
    <activity>
      <statement>
        <p>
          Find the intersection of the line <m>x - y + 4 = 0</m> and the
          hyperbola <m>\frac{x^2}{1} - \frac{y^2}{4} = 1</m>. 
        </p>
      </statement>
      <solution>
        <p>
          Solving for intesection is algebraically the same as solving
          the system of two equations. In the first equation,
          we can isolate <m>y</m> to get <m>y = x+4</m>. We can
          use this to replace <m>y</m> in the equation of the
          hyperbola.
          <md>
            <mrow>
            x^2 - \frac{1}{4} (x+4)^2 \amp = 1 
            </mrow>
            <mrow>
            4x^2 - (x+4)^2 \amp = 4 
            </mrow>
            <mrow>
            4x^2 - x^2 - 8x - 16 \amp = 4 
            </mrow>
            <mrow>
            3x^2  - 8x - 20 \amp = 0 
            </mrow>
          </md>
          This is a quadratic; the quadratic equation tells us the
          roots.
          <me>
            x = \frac{8 \pm \sqrt{64 + 240}}{6} = \frac{8 \pm
            2\sqrt{76}}{6} = \frac{4 \pm \sqrt{76}}{3}
          </me>
          Then we can use the previous <m>y = x+4</m> to get the
          matching <m>y</m> coordinates. 
          <me>
            y = x + 4 \frac{4 \pm \sqrt{76}}{3} + 4 = \frac{16 \pm
            \sqrt{76}}{3} 
          </me>
          All together, we have two intersection points. 
          <md>
            <mrow>
            \amp \left( \frac{4 + \sqrt{76}}{3}, \frac{16 + \sqrt{76}}{3}
            \right) 
            </mrow>
            \amp \left( \frac{4 - \sqrt{76}}{3}, \frac{16 - \sqrt{76}}{3}
            \right) 
            <mrow>
            </mrow>
          </md>
          We could write the decimal approximates of these values.
          That might help us know where to draw them, but the above
          expressions are preferable as exact values.  
        </p>
      </solution>
    </activity>
  </subsection>
  <subsection xml:id="week1-concepts">
    <title>Conceptual Review Questions</title>
    <p>
      <ul>
        <li>
          What data determine a line? What is the minimum information
          we need?
        </li>
        <li>
          What does slope mean and how is it measured?
        </li>
        <li>
          What is a conic? Why are the four shapes (circle, parabola,
          ellipse and hyperbola) considered four members of the same
          family. 
        </li>
        <li>
          In geometry, intersection is where two geometric shapes
          meet. What does intersection mean algebraically?
        </li>
      </ul>
    </p>
  </subsection>
</section>
